theories/iris/examples/effects/coroutines.v
@@ -1336,7 +1336,7 @@ Section yield_par.
           
             
             
-
+End yield_par.
         
         
         
